\documentclass[letterpaper]{article}
\usepackage[square,sort,comma,numbers]{natbib}
\usepackage{array}
%====================================================================%
\input{scufftex}
\graphicspath{{figures/}}
\renewcommand{\wt}{\widetilde}

%------------------------------------------------------------
%------------------------------------------------------------
%- Special commands for this document -----------------------
%------------------------------------------------------------
%------------------------------------------------------------

%------------------------------------------------------------
%------------------------------------------------------------
%- Document header  -----------------------------------------
%------------------------------------------------------------
%------------------------------------------------------------
\title {Electrostatic Green's function above dielectric substrate
        and ground plane 
       }
\author {Homer Reid}
\date {March 2, 2017}

%------------------------------------------------------------
%------------------------------------------------------------
%- Start of actual document
%------------------------------------------------------------
%------------------------------------------------------------

\begin{document}
\pagestyle{myheadings}
\markright{Homer Reid: Electrostatic GF above PCB} 
\maketitle

\tableofcontents

\subsection{2D Fourier representation of free-space Green's function}

The 3D Fourier representation of the free-space Green's function---the
potential at $\vb x=(\vbrho,z)$ due to a point charge at 
$\vb x^\prime=(\vbrho^\prime,z^\prime)$---is 
%====================================================================%
\begin{align*}
G_0(\vbrho, z; \vbrho^\prime, z^\prime)
=
 \frac{1}{4\pi |\vb x-\vb x^\prime|}
 &=\int \frac{d^3 \vb k}{(2\pi)^3}
        \frac{e^{i\vb k \cdot (\vb x-\vb x^\prime)}}{|\vb k|^2}
\intertext{Evaluate the $k_z$ integral:}
 &=\frac{1}{2}\int \frac{d^2 \vb q}{(2\pi)^2}
        \frac{e^{i\vb q\cdot (\vbrho-\vbrho^\prime)-q|z-z^\prime|}}{q},
 \qquad  \vb   q\equiv  \vb k_\parallel,
 \quad        q\equiv |\vb q|.
\end{align*}
%====================================================================%

\subsection{Potential due to a surface-charge layer at $z=T$}

%====================================================================%
\begin{align*}
 \Phi(\vbrho, z)
   &=\int \, G_0(\vbrho,z; \vb y, T)\, \sigma(\vb y) \, d^2 \vb y
\\
   &=\frac{1}{2} \int \frac{d^2 \vb q}{(2\pi)^2}
     \frac{e^{i\vb q \cdot \vbrho - q|z-T|}}{q}
     \underbrace{\int d\vb y \, \sigma(\vb y) \, e^{-i\vb q \cdot \vb y}}
               _{\wt{\sigma}(\vb q)}
\\
   &=\int \frac{d^2 \vb q}{(2\pi)^2}
     \frac{\wt\sigma(\vb y)e^{i\vb q \cdot \vbrho - q|z-T|}}{2q}
\end{align*}
%====================================================================%

\subsection{Potential at $(\vbrho, z)$ due to point charge at
            $(\vbrho^\prime, z^\prime)$ 
            above dielectric interface at $z=T$ and ground plane at $z=0$}

Here I assume $z^\prime>T$, i.e. the point charge lies above the dielectric
layer.

Potential and its $z$-derivative above dielectric layer $(z>T)$:
%====================================================================%
\begin{align}
 G\sups{above}(\vbrho, z; \vbrho^\prime, z^\prime)
  &=\frac{1}{4\pi\sqrt{|\vbrho-\vbrho^\prime|^2 + (z-z^\prime)^2}}
   -\frac{1}{4\pi\sqrt{|\vbrho-\vbrho^\prime|^2 + (z+z^\prime)^2}}
\\
%--------------------------------------------------------------------%
 &\qquad+ \int \frac{d^2 \vb q}{(2\pi)^2}
          \frac{\wt \sigma(\vb q)e^{i\vb q \cdot (\vbrho-\vbrho^\prime)-qz}}{q}\sinh qT
\\[5pt]
%--------------------------------------------------------------------%
 -\partial_z
G\sups{above}(\vbrho, z; \vbrho^\prime, z^\prime)
  &= \frac{(z-z^\prime)}{4\pi\big[|\vbrho-\vbrho^\prime|^2 + (z-z^\prime)^2\big]^{3/2}}
    -\frac{(z+z^\prime)}{4\pi\big[|\vbrho-\vbrho^\prime|^2 + (z+z^\prime)^2\big]^{3/2}}
\\
%--------------------------------------------------------------------%
  &\qquad+ \int \frac{d^2 \vb q}{(2\pi)^2}
          \wt \sigma(\vb q)e^{i\vb q \cdot (\vbrho-\vbrho^\prime)-qz}\sinh qT
\label{dzdGAbove}
\end{align}
%====================================================================%
\noindent Potential and $z$-derivative inside dielectric layer $(0<z<T)$:
%====================================================================%
\begin{align}
 G\sups{inside}(\vbrho, z; \vbrho^\prime, z^\prime)
  &=\frac{1}{4\pi\sqrt{|\vbrho-\vbrho^\prime|^2 + (z-z^\prime)^2}}
   -\frac{1}{4\pi\sqrt{|\vbrho-\vbrho^\prime|^2 + (z+z^\prime)^2}}
\\
%--------------------------------------------------------------------%
 &\qquad+\int \frac{d^2 \vb q}{(2\pi)^2}
          \frac{\wt \sigma(\vb q)e^{i\vb q \cdot (\vbrho-\vbrho^\prime)-qT}}{q}\sinh qz
\\[5pt]
%--------------------------------------------------------------------%
-\partial_z G\sups{inside}(\vbrho, z; \vbrho^\prime, z^\prime)
  &= \frac{(z-z^\prime)}{4\pi\big[|\vbrho-\vbrho^\prime|^2 + (z-z^\prime)^2\big]^{3/2}}
    -\frac{(z+z^\prime)}{4\pi\big[|\vbrho-\vbrho^\prime|^2 + (z+z^\prime)^2\big]^{3/2}}
%--------------------------------------------------------------------%
\\
  &\qquad- \int \frac{d^2 \vb q}{(2\pi)^2}
          \wt \sigma(\vb q)e^{i\vb q \cdot (\vbrho-\vbrho^\prime)-qT}\cosh qz
\label{dzdGBelow}
%--------------------------------------------------------------------%
\end{align}
%====================================================================%
Boundary condition at $z=T$:
%====================================================================%
$$            \left|\pard{G\sups{above}}{z}\right|_{z=T} = 
   \epsilon_r \left|\pard{G\sups{inside}}{z}\right|_{z=T} 
$$
%====================================================================%
Insert (\ref{dzdGAbove}) and (\ref{dzdGBelow}):
%====================================================================%
\begin{align*}
&\hspace{-0.2in}
\int \Upsilon(\epsilon_r,T,q) \wt\sigma(\vb q) e^{i\vb q \cdot (\vbrho-\vbrho^\prime)} 
\, \frac{d\vb q}{(2\pi)^2}
\\
&=\frac{\epsilon_r-1}{4\pi}
   \left[\frac{(z^\prime-T)}
           {\big\{ |\vbrho-\vbrho^\prime|^2 + (z^\prime-T)^2\big\}^{3/2}}
        -\frac{(z^\prime+T)}
           {\big\{ |\vbrho-\vbrho^\prime|^2 + (z^\prime+T)^2\big\}^{3/2}}
   \right]
\end{align*}
or, inverting the Fourier transform,
%====================================================================%
\begin{align*}
\wt \sigma(\vb q)
&=\frac{\epsilon_r-1}{4\pi\Upsilon(\epsilon_r, T, q)}
  \int e^{-i\vb q \cdot (\vbrho-\vbrho^\prime)}
   \left[\frac{(z^\prime-T)}
           {\big\{ |\vbrho-\vbrho^\prime|^2 + (z^\prime-T)^2\big\}^{3/2}}
        -\frac{(z^\prime+T)}
           {\big\{ |\vbrho-\vbrho^\prime|^2 + (z^\prime+T)^2\big\}^{3/2}}
   \right]
  \,d\vbrho
\end{align*}
%====================================================================%
where I put
%====================================================================%
$$ \Upsilon(\epsilon_r, T, q) \equiv
   e^{-qT}\Big[\sinh qT + \epsilon_r \cosh qT\Big].
$$
%====================================================================%
To evaluate the integrals, I go like this:
%====================================================================%
\begin{align*} 
 \mc I(\vb q, \Delta) 
&= 
 \int \frac{\Delta}{ \big[|\vb u|^2 + \Delta^2\big]^{3/2}}
  e^{i\vb q \cdot \vb u} \, d\vb u
\\
&= \int_0^\infty \frac{u\,du}{\big[u^2 + \Delta^2\big]^{3/2}}
   \int_0^{2\pi} e^{-i q u \cos\theta}\,d\theta 
\\
&= 2\pi \int_0^\infty \frac{u\,du}{\big[u^2 + \Delta^2\big]^{3/2}}J_0(qu)
\\
&= 2\pi e^{-q\Delta}.
\end{align*}
%====================================================================%
Then I have
%====================================================================%
\begin{align*}
 \wt{\sigma}(\vb q)
 &=\frac{\epsilon_r-1}{2e^{-qT}\big[\sinh qT + \epsilon_r \cosh qT\big]}
    \Big[ e^{-q(z^\prime-T)} - e^{-q(z^\prime+T)}\Big]
\\
&=
 \frac{ (\epsilon_r-1)\sinh qT }{ \sinh qT + \epsilon_r \cosh qT}
 e^{-q(z^\prime - T)}
\end{align*}
   
%====================================================================%

\end{document}
